{
 "cells": [
  {
   "cell_type": "code",
   "execution_count": 4,
   "metadata": {},
   "outputs": [],
   "source": [
    "#=\n",
    "Consider carbon dioxide, a triatomic linear molecule with a carbon atom at the center which is \n",
    "double-bonded to two oxygen atoms. We can model as a system of springs and masses, shown below.\n",
    "\n",
    "      spring          spring\n",
    "O <---/////---> C <---/////---> O\n",
    "|               |               |   \n",
    "|--> x1         |--> x2         |--> x3\n",
    "\n",
    "Where:\n",
    "O: Oxygen atom\n",
    "C: Carbon atom\n",
    "///: Spring representing the double bond\n",
    "x1, x2, x3: Positions of the respective atoms\n",
    "=#"
   ]
  },
  {
   "attachments": {},
   "cell_type": "markdown",
   "metadata": {},
   "source": [
    "Using Newton's second law, we have 3 equations for the 3 mass system: \n",
    "$$\n",
    "\\begin{aligned}\n",
    "m_1 \\ddot{x_1} &= k(x_2 - x_1) \\\\\n",
    "m_2 \\ddot{x_2} &= k(x_3 - x_2) - k(x_2 - x_1) \\\\\n",
    "m_3 \\ddot{x_3} &= -k(x_3 - x_2)\n",
    "\\end{aligned}\n",
    "$$\n",
    "We make the ansatz $ x_j = A_j e^{i \\omega t}$, where mass index $j = (1,2,3)$ since we have three atoms. Differentating, \n",
    "$$\n",
    "\\begin{aligned}\n",
    "x_j &= A_j e^{i \\omega t} \\\\\n",
    "\\dot{x_j} &= i \\omega A_j e^{i \\omega t} \\\\\n",
    "\\ddot{x_j}&= -\\omega^2 A_j e^{i \\omega t}\n",
    "\\end{aligned}\n",
    "$$\n",
    "Substituting into the equtions of motion, \n",
    "$$\n",
    "\\begin{aligned}\n",
    "m_1(-\\omega^2 A_1 e^{iwt}) &= k (A_2 e^{iwt} - A_1 e^{iwt}) \\\\\n",
    "m_2(-\\omega^2 A_2 e^{iwt}) &= k (A_3 e^{iwt} - A_2 e^{iwt}) - k (A_2 e^{iwt} - A_1 e^{iwt}) \\\\\n",
    "m_3(-\\omega^3 A_3 e^{iwt}) &= -k (A_3 e^{iwt} - A_2 e^{iwt})\n",
    "\\end{aligned}\n",
    "$$\n",
    "Cancelling the common $e^{iwt}$ and rearranging, \n",
    "$$\n",
    "\\begin{aligned}\n",
    "(-m_1 \\omega^2 + k)A_1 - kA_2 + 0 \\cdot A_3 &= 0 \\\\\n",
    "kA_1 + (-m_2 \\omega^2 + 2k)A_2 - kA_3 &= 0 \\\\\n",
    "0 \\cdot A_1 - kA_2 + (-m_3 \\omega^2 + k) &= 0\n",
    "\\end{aligned}\n",
    "$$\n",
    "Expressing the system in matrix form, \n",
    "$$\n",
    "\\begin{bmatrix}\n",
    "-m_1\\omega^2+k & -k  & 0 \\\\\n",
    "-k & -m_2 \\omega^2 + 2k & -k \\\\\n",
    "0 & -k & -m_3\\omega^2 + k\n",
    "\\end{bmatrix} \\begin{bmatrix}\n",
    "A_1 \\\\ A_2 \\\\ A_3 \n",
    "\\end{bmatrix} = 0\n",
    "$$\n",
    "Let $m_1 = m_3 = M$, and $m_2 = m$ to simplify notation. Setting the determinant of the 3x3 to matrix gives the charecteristic equation. The roots of this polynomial gives values for $\\omega^2$ for which there exist non-trivial solutions to the system of equations. Taking the square root gives values of $\\omega$, the angular frequencies corresponding to each normal mode. \n",
    "$$\n",
    "det\\left(\\begin{bmatrix}\n",
    "-M\\omega^2+k & -k  & 0 \\\\\n",
    "-k & -m \\omega^2 + 2k & -k \\\\\n",
    "0 & -k & -M\\omega^2 + k\n",
    "\\end{bmatrix} \\right) = 0 \n",
    "$$\n",
    "$$\n",
    "(-M\\omega^2 + k)\\left( (-m\\omega^2 + 2k)(-M\\omega^2 + k) - k^2\\right)+k\\left( -k(-M\\omega^2 + k \\right)) = 0\n",
    "$$\n",
    "$$\n",
    "(-m\\omega^2)(-M\\omega^2 + k)\\left(-M\\omega^2 + k\\left(1+\\frac{2M}{m}\\right)\\right) = 0\n",
    "$$\n",
    "We find three eigenvalues and angular frequencies: \n",
    "$$\n",
    "\\omega_1^2 = 0, \\;\\; \\; \\omega_2^2 = \\frac{k}{M},\\;\\; \\; \\omega_3^2 = \\frac{k(1 + \\frac{2M}{m}}{M}\n",
    "$$\n",
    "$$\n",
    "\\omega_1 = 0, \\;\\; \\;  \\omega_2 = \\sqrt{\\frac{k}{M}}, \\;\\; \\;   \\omega_3 = \\sqrt{\\frac{k(1 + \\frac{2M}{m}}{M}}\n",
    "$$\n",
    "For the **first normal mode**, substititng the eigenvector $\\omega_1^2 = 0$ into the matrix equation, \n",
    "$$\n",
    "\\begin{bmatrix}\n",
    "k & -k & 0 \\\\\n",
    "-k & 2k & -k \\\\\n",
    "0 & -k & k\n",
    "\\end{bmatrix}\\begin{bmatrix}\n",
    "A_1 \\\\ A_2 \\\\ A_3 \\end{bmatrix} = 0\n",
    "$$\n",
    "$$\n",
    "\\begin{aligned}\n",
    "kA_1 - kA_2 &= 0 \\quad (1) \\\\\n",
    "-kA_1 + 2kA_2 - kA_3 &= 0 \\quad (2) \\\\\n",
    "-kA_2 + kA_3 &= 0 \\quad (3)\n",
    "\\end{aligned} \\rightarrow e_1 = \\begin{bmatrix} 1 \\\\ 1 \\\\1 \\end{bmatrix}  \n",
    "$$\n",
    "We see that $A_1 = A_2$ and $A_2 = A_3$ from Eq. 1 and Eq. 3, respectively. As $A_1 = A_2 = A_3$, Eq. 2 is always satisified, so their amplitudes must always be equal. These corresponds to a pendular mode, with the position and velocity of each atom being the same at any given time. \n",
    "\n",
    "For the **second normal mode**, substituting $\\omega_2^2 = \\frac{k}{M}$ into the matrix equation,\n",
    "$$\n",
    "\\begin{bmatrix}\n",
    "-M\\left(\\frac{k}{M}\\right)+k & -k & 0 \\\\\n",
    "-k & -m\\left(\\frac{k}{M}\\right)+2k & -k \\\\\n",
    "0 & -k & -M\\left(\\frac{k}{M}\\right)+k\n",
    "\\end{bmatrix}\n",
    "\\begin{bmatrix}\n",
    "A_1 \\\\ A_2 \\\\ A_3\n",
    "\\end{bmatrix}\n",
    "= \\begin{bmatrix}\n",
    "0 & -k & 0 \\\\\n",
    "-k & k\\left(2 - \\frac{m}{M}\\right) & -k \\\\\n",
    "0 & -k & 0\n",
    "\\end{bmatrix}\n",
    "\\begin{bmatrix}\n",
    "A_1 \\\\ A_2 \\\\ A_3\n",
    "\\end{bmatrix} = 0\n",
    "$$\n",
    "$$\n",
    "\\begin{aligned}\n",
    "-kA_2 &= 0 \\quad (1) \\\\\n",
    "-kA_1 + k\\left(2 - \\frac{m}{M}\\right)A_2 - kA_3 &= 0 \\quad (2) \\\\\n",
    "-kA_2 &= 0 \\quad (3)\n",
    "\\end{aligned} \\rightarrow e_2 = \\begin{bmatrix} 1 \\\\ 0 \\\\ -1 \\end{bmatrix}\n",
    "$$\n",
    "Eq. 1 and Eq. 3 suggest that $A_2 = 0$, and substituing this into Eq. 2 gives $-kA_1 - kA_3 = 0$. Therefore, $A_1 = -A_3$. In this mode, the Oxygen atoms (outer masses) moves with equal amplitude in opposite directions, while the Carbon atom (center mass) remains stationary. \n",
    "\n",
    "\n",
    "For the **third normal mode**, substituing $\\omega_3^2 = \\frac{k(1 + \\frac{2M}{m})}{M}$ into the matrix equation, \n",
    "\n",
    "$$\n",
    "\\begin{bmatrix}\n",
    "-k(1+\\frac{2M}{m}) & -k & 0 \\\\\n",
    "-k & -k(1+\\frac{2M}{m}) & -k \\\\\n",
    "0 & -k & -k(1+\\frac{2M}{m})\n",
    "\\end{bmatrix}\n",
    "\\begin{bmatrix}\n",
    "A_1 \\\\ A_2 \\\\ A_3\n",
    "\\end{bmatrix}\n",
    "= 0\n",
    "$$\n",
    "$$\n",
    "\\begin{aligned}\n",
    "-k\\left(1+\\frac{2M}{m}\\right)A_1 - kA_2 &= 0 \\quad (1) \\\\\n",
    "-kA_1 - k\\left(1+\\frac{2M}{m}\\right)A_2 - kA_3 &= 0 \\quad (2) \\\\\n",
    "-kA_2 - k\\left(1+\\frac{2M}{m}\\right)A_3 &= 0 \\quad (3) \n",
    "\\end{aligned} \\rightarrow e_3 = \\begin{bmatrix}\n",
    "-\\frac{1}{1+\\frac{2M}{m}} \\\\\n",
    "1 \\\\\n",
    "-\\frac{1}{1+\\frac{2M}{m}}\n",
    "\\end{bmatrix}\n",
    "$$\n",
    "\n",
    "Eq. 1 gives $A_1 = -\\frac{1}{1+\\frac{2M}{m}} A_2$. Eq. 3 gives $A_3 = -\\frac{1}{1+\\frac{2M}{m}} A_2$. Substituting into Eq. 2 confirms this, and $A_2$ is our free variable. In this mode, the central mass moves in a one direction while each outer mass moves in the opposite direction with smaller amplitudes dictated by the mass ratio $\\frac{M}{m}$. \n",
    "\n",
    "Assuming Carbon is $^{12}C$ and Oxygen is $^{16}O$, $m = 1.993 \\cdot 10^{-26} kg$, $M = 2.66\\cdot 10^{-26}kg$, and $k=3628 N/m$, we can calculate values. "
   ]
  },
  {
   "cell_type": "code",
   "execution_count": 3,
   "metadata": {},
   "outputs": [
    {
     "name": "stdout",
     "output_type": "stream",
     "text": [
      "Angular Frequencies:\n",
      "ω₁ = 0\n",
      "ω₂ = 3.6931149107983225e14\n",
      "ω₃ = 7.074356771843592e14\n",
      "\n",
      "Normal Modes (Eigenvectors):\n",
      "e₁ = [1, 1, 1]\n",
      "e₂ = [1, 0, -1]\n",
      "e₃ = [-0.27252837412826475, 1.0, -0.27252837412826475]\n"
     ]
    }
   ],
   "source": [
    "m = 1.993e-26   # mass of Carbon atom in kg\n",
    "M = 2.66e-26    # mass of Oxygen atom in kg\n",
    "k = 3628        # spring constant in N/m\n",
    "\n",
    "ω₁ = 0\n",
    "ω₂= √(k / M)\n",
    "ω₃ = √(k * (1 + 2M / m) / M)\n",
    "\n",
    "e₁ = [1, 1, 1]\n",
    "e₂ = [1, 0, -1]\n",
    "e₃ = [-1 / (1 + 2M / m), 1, -1 / (1 + 2M / m)]\n",
    "\n",
    "println(\"Angular Frequencies:\")\n",
    "println(\"ω₁ = \", ω₁)\n",
    "println(\"ω₂ = \", ω₂)\n",
    "println(\"ω₃ = \", ω₃)\n",
    "\n",
    "println(\"\\nNormal Modes (Eigenvectors):\")\n",
    "println(\"e₁ = \", e₁)\n",
    "println(\"e₂ = \", e₂)\n",
    "println(\"e₃ = \", e₃)"
   ]
  },
  {
   "attachments": {},
   "cell_type": "markdown",
   "metadata": {},
   "source": [
    "In summary, \n",
    "\n",
    "1st normal mode: ω₁ = 0 and e₁ = [1, 1, 1]. All atoms are in phase, so the masses move together rigidly, with no restoring force. \n",
    "\n",
    "2nd normal mode: ω₂ = 3.693e14 rad/s and e₂ = [1, 0, -1]. The outer atoms move out of phase, while the middle atom remains stationary. \n",
    "\n",
    "3rd normal mode: ω₃ = 7.074e14 rad/s and e₃ = [-0.272, 1, -0.272]. The middle atom moves in one direction, while the outer atoms move in the opposite direction with smaller amplitude. \n",
    "\n",
    "The high frequency is reasonable for molecular vibrations. "
   ]
  },
  {
   "cell_type": "markdown",
   "metadata": {},
   "source": []
  }
 ],
 "metadata": {
  "kernelspec": {
   "display_name": "Julia 1.8.5",
   "language": "julia",
   "name": "julia-1.8"
  },
  "language_info": {
   "file_extension": ".jl",
   "mimetype": "application/julia",
   "name": "julia",
   "version": "1.8.5"
  },
  "orig_nbformat": 4
 },
 "nbformat": 4,
 "nbformat_minor": 2
}
